src/ASN1/ASN1.Spec.ILC.fst
@@ -5,6 +5,8 @@ open ASN1.Base
 open ASN1.Spec.IdentifierU32
 open ASN1.Spec.LengthU32
 
+open ASN1.Spec.Content.OCTETSTRING
+
 open LowParse.Spec.Base
 open LowParse.Spec.Combinators
 open LowParse.Spec.VLGen
@@ -51,6 +53,25 @@ let parser_asn1_ILC_twin_case_injective
 : Lemma
   (and_then_cases_injective (parse_asn1_ILC_twin id p))
 = and_then_cases_injective_intro (parse_asn1_ILC_twin id p) (fun id1 id2 _ _ -> assert (id1 = id) ; assert (id2 = id))
+
+let parse_asn1_anyILC
+: asn1_strong_parser (asn1_t (ASN1_ANY_ILC))
+= parse_asn1_identifier_U32 `nondep_then` (parse_asn1_LC #(ASN1_TERMINAL ASN1_OCTETSTRING) parse_asn1_octetstring)
+
+let parse_asn1_anyILC_twin
+: asn1_id_t -> asn1_strong_parser (asn1_t (ASN1_ANY_ILC))
+= fun id -> (parse_ret id) `nondep_then` (parse_asn1_LC #(ASN1_TERMINAL ASN1_OCTETSTRING) parse_asn1_octetstring)
+
+let parse_asn1_anyILC_twin_and_then_cases_injective ()
+: Lemma (and_then_cases_injective parse_asn1_anyILC_twin)
+= let p = parse_asn1_anyILC_twin in
+  and_then_cases_injective_intro p (fun x1 x2 b1 b2 -> 
+    let p1 = parse_ret x1 in
+    let p2 = parse_ret x2 in
+    let p' = (parse_asn1_LC #(ASN1_TERMINAL ASN1_OCTETSTRING) parse_asn1_octetstring) in
+    nondep_then_eq p1 p' b1;
+    nondep_then_eq p2 p' b2
+  )
 
 (*
 
