src/ASN1/ASN1.Syntax.fst
@@ -1,0 +1,209 @@
+module ASN1.Syntax
+
+open ASN1.Base
+
+module U32 = FStar.UInt32
+module List = FStar.List.Tot
+module T = FStar.Tactics
+
+// for identifiers
+
+let mk_constant_id (x : UInt.uint_t 32) : asn1_id_t
+= MK_ASN1_ID UNIVERSAL PRIMITIVE (U32.uint_to_t x)
+
+let mk_constant_constructed_id (x : UInt.uint_t 32) : asn1_id_t
+= MK_ASN1_ID UNIVERSAL CONSTRUCTED (U32.uint_to_t x)
+
+let mk_custom_id (c : asn1_id_class_t) (f : asn1_id_flag_t) (x : UInt.uint_t 32) : asn1_id_t
+= MK_ASN1_ID c f (U32.uint_to_t x)
+
+// for OID definitions
+
+let rec mk_u32list (l : list (UInt.uint_t 32)) : list U32.t
+= match l with
+  | [] -> []
+  | hd :: tl -> (U32.uint_to_t hd) :: (mk_u32list tl)
+
+let mk_oid (l : list (UInt.uint_t 32)) : Pure (asn1_oid_t)
+  (requires asn1_OID_wf (mk_u32list l))
+  (ensures fun _ -> True)
+= mk_u32list l
+
+let mk_oid_app (oid : asn1_oid_t) (x : UInt.uint_t 32) : asn1_oid_t
+= List.append oid [U32.uint_to_t x]
+
+let op_Slash_Plus = mk_oid_app
+
+// for choices
+
+let is_ILC (#s) (x : asn1_k s)
+= match x with
+  | ASN1_ILC _ _ -> true
+  | _ -> false
+
+let proj_identifier (#s) (x : asn1_k s {is_ILC x}) 
+= match x with
+  | ASN1_ILC id c -> id
+
+let proj_content (#s) (x : asn1_k s {is_ILC x}) 
+= match x with
+  | ASN1_ILC id c -> c
+
+let mk_prefixed (id : asn1_id_t) (#s) (x : asn1_k s)
+= ASN1_ILC id (ASN1_PREFIXED x)
+
+let mk_retagged (id : asn1_id_t) (#s) (x : asn1_k s {is_ILC x})
+= ASN1_ILC id (proj_content x)
+
+let op_Star_Hat (name : string) (#t) (x : t)
+= x
+
+let op_Hat_Star (name : string) (#s) (x : asn1_k s {is_ILC x}) : (asn1_id_t * asn1_content_k)
+= match x with
+  | ASN1_ILC id c -> (id, c)
+
+let no_repeats_by_norm () =  T.norm [delta;zeta;primops;iota]; T.trefl ()
+
+let asn1_choice (ls : list (asn1_id_t * asn1_content_k)) (#[no_repeats_by_norm() ] pf : squash (List.noRepeats (List.map fst ls) ))
+= ASN1_CHOICE_ILC ls pf
+
+// for sequences
+
+let is_terminal (#s) (x : asn1_k s)
+= if is_ILC x then
+    match (proj_content x) with
+    | ASN1_TERMINAL _ -> true
+    | _ -> false
+  else
+    false
+
+let proj_terminal_k (#s) (x : asn1_k s {is_terminal x})
+= match proj_content x with
+  | ASN1_TERMINAL tk -> tk
+
+let proj_terminal_t (#s) (x : asn1_k s {is_terminal x})
+= match proj_content x with
+  | ASN1_TERMINAL tk -> asn1_terminal_t tk
+
+let mk_default_field (#s) (x : asn1_k s {is_terminal x}) (v : proj_terminal_t x)
+= ASN1_DEFAULT_TERMINAL (proj_identifier x) #(proj_terminal_k x) v
+
+let mk_restricted_default_field (#s) (x : asn1_k s {is_terminal x}) (f : proj_terminal_t x -> bool) (v : proj_terminal_t x {f v})
+= ASN1_DEFAULT_RESTRICTED_TERMINAL (proj_identifier x) #(proj_terminal_k x) f v
+
+let mk_restricted_field (#s) (x : asn1_k s {is_terminal x}) (f : proj_terminal_t x -> bool)
+= ASN1_ILC (proj_identifier x) (ASN1_RESTRICTED_TERMINAL (proj_terminal_k x) f)
+
+let field_type (s : Set.set asn1_id_t) (d : asn1_decorator) 
+= match d with
+  | DEFAULT -> asn1_decorated_k s d
+  | _ -> asn1_k s
+
+let op_Hat_Colon (#s : Set.set asn1_id_t)  
+  (d : asn1_decorator) 
+  (f : field_type s d)
+: asn1_gen_item_k
+= match d with
+  | DEFAULT -> mk_ASN1_GEN_ITEM #s #d f
+  | PLAIN -> mk_ASN1_GEN_ITEM (ASN1_PLAIN_ILC #s f)
+  | OPTION -> mk_ASN1_GEN_ITEM (ASN1_OPTION_ILC #s f)
+
+let seq_wf_by_norm_smt () =  T.norm [delta;zeta;primops;iota]; T.smt ()
+
+let mk_gen_items (items : list asn1_gen_item_k) (#[seq_wf_by_norm_smt ()] pf : squash (asn1_sequence_k_wf (List.map (fun x -> let (| s, d, _ |) = x in (s, d) ) items))) : asn1_gen_items_k
+= (| items, pf |)
+
+// constants
+
+let boolean_id = mk_constant_id 1
+
+let asn1_boolean = ASN1_ILC boolean_id (ASN1_TERMINAL ASN1_BOOLEAN)
+
+let integer_id = mk_constant_id 2
+
+let asn1_integer = ASN1_ILC integer_id (ASN1_TERMINAL ASN1_INTEGER)
+
+let bit_string_id = mk_constant_id 3
+
+let asn1_bitstring = ASN1_ILC boolean_id (ASN1_TERMINAL ASN1_BITSTRING)
+
+let octetstring_id = mk_constant_id 4
+
+let asn1_octetstring = ASN1_ILC octetstring_id (ASN1_TERMINAL ASN1_OCTETSTRING)
+
+let null_id = mk_constant_id 5
+
+let asn1_null = ASN1_ILC null_id (ASN1_TERMINAL ASN1_NULL)
+
+let oid_id = mk_constant_id 6
+
+let asn1_oid = ASN1_ILC oid_id (ASN1_TERMINAL ASN1_OID)
+
+let utf8string_id = mk_constant_id 12
+
+let asn1_utf8string = ASN1_ILC utf8string_id (ASN1_TERMINAL ASN1_UTF8STRING)
+
+let sequence_id = mk_constant_constructed_id 16
+
+let asn1_sequence (items : list asn1_gen_item_k) (#[seq_wf_by_norm_smt ()] pf : squash (asn1_sequence_k_wf (List.map (fun x -> let (| s, d, _ |) = x in (s, d) ) items)))
+= ASN1_ILC sequence_id (ASN1_SEQUENCE (| items, pf |))
+
+let asn1_sequence_of (#s) (item : asn1_k s) = ASN1_ILC sequence_id (ASN1_SEQUENCE_OF item)
+
+let set_id = mk_constant_constructed_id 17
+
+let asn1_set_of (#s) (item : asn1_k s) = ASN1_ILC set_id (ASN1_SET_OF item)
+
+let printablestring_id = mk_constant_id 19
+
+let asn1_printablestring = ASN1_ILC printablestring_id (ASN1_TERMINAL ASN1_PRINTABLESTRING)
+
+let teletexstring_id = mk_constant_id 20
+
+let asn1_teletexstring = ASN1_ILC teletexstring_id (ASN1_TERMINAL ASN1_OCTETSTRING)
+
+let ia5string_id = mk_constant_id 22
+
+let asn1_ia5string = ASN1_ILC ia5string_id (ASN1_TERMINAL ASN1_OCTETSTRING)
+
+let utctime_id = mk_constant_id 23
+
+let asn1_utctime = ASN1_ILC utctime_id (ASN1_TERMINAL ASN1_UTCTIME)
+
+let generalizedtime_id = mk_constant_id 24
+
+let asn1_generalizedtime = ASN1_ILC generalizedtime_id (ASN1_TERMINAL ASN1_GENERALIZEDTIME)
+
+let visiblestring_id = mk_constant_id 26
+
+let asn1_visiblestring = ASN1_ILC visiblestring_id (ASN1_TERMINAL ASN1_OCTETSTRING)
+
+let universalstring_id = mk_constant_id 28
+
+let asn1_universalstring = ASN1_ILC universalstring_id (ASN1_TERMINAL ASN1_OCTETSTRING)
+
+let bMPstring_id = mk_constant_id 30
+
+let asn1_bMPstring = ASN1_ILC bMPstring_id (ASN1_TERMINAL ASN1_OCTETSTRING)
+
+// for any
+
+let asn1_any = ASN1_ANY_ILC
+
+let asn1_any_oid 
+  (name : string)
+  (supported : list (asn1_oid_t * asn1_gen_items_k)) 
+  (fallback : option asn1_gen_items_k)
+  (#[seq_wf_by_norm_smt ()] pfwf : squash (asn1_sequence_k_wf (List.append (List.map (fun x -> let (| s, d, _ |) = x in (s, d)) []) [(Set.singleton oid_id, PLAIN)])))
+  (#[no_repeats_by_norm ()] pfsup : squash (List.noRepeats (List.map fst supported)))
+= ASN1_ILC sequence_id (ASN1_ANY_DEFINED_BY [] oid_id ASN1_OID supported fallback pfwf pfsup)
+
+let ans1_any_oid_prefix
+  (prefix : list asn1_gen_item_k)
+  (name : string)
+  (supported : list (asn1_oid_t * asn1_gen_items_k)) 
+  (fallback : option asn1_gen_items_k)
+  (#[seq_wf_by_norm_smt ()] pfwf : squash (asn1_sequence_k_wf (List.append (List.map (fun x -> let (| s, d, _ |) = x in (s, d)) prefix) [(Set.singleton oid_id, PLAIN)])))
+  (#[no_repeats_by_norm ()] pfsup : squash (List.noRepeats (List.map fst supported)))
+= ASN1_ILC sequence_id (ASN1_ANY_DEFINED_BY prefix oid_id ASN1_OID supported fallback pfwf pfsup)
+
